theory/x64Semantics.thy
@@ -10,7 +10,8 @@ begin
 
 text \<open> define our x64 semantics in Isabelle/HOL, following the style of CompCert x64 semantics: https://github.com/AbsInt/CompCert/blob/master/x86/Asm.v  \<close>
 
-type_synonym regset = "ireg \<Rightarrow> u64"
+
+type_synonym regset = "preg \<Rightarrow> u64"
 
 syntax "_pregmap_set" :: "'a => 'b => 'c => 'a" ("_ # _ <- _" [1000, 1000, 1000] 1)
 
@@ -18,8 +19,7 @@ syntax "_pregmap_set" :: "'a => 'b => 'c => 'a" ("_ # _ <- _" [1000, 1000, 1000]
 translations
   "_pregmap_set a b c" => "(a(b := c))"
 
-
-fun undef_regs :: "ireg list \<Rightarrow> regset \<Rightarrow> regset" where
+fun undef_regs :: "preg list \<Rightarrow> regset \<Rightarrow> regset" where
 "undef_regs [] rs = rs" |
 "undef_regs (r#l') rs = undef_regs l' (rs#r <- 0)"
 
@@ -27,53 +27,126 @@ datatype outcome = Next u64 regset mem | Stuck
 
 definition exec_ret :: "memory_chunk \<Rightarrow> mem \<Rightarrow> regset \<Rightarrow> outcome" where
 "exec_ret chunk m rs = (
-  let nsp =  (rs SP) + (u64_of_memory_chunk chunk) in
+  let nsp =  (rs (IR SP)) + (u64_of_memory_chunk chunk) in
     case Mem.loadv M64 m (Vlong nsp) of
     None \<Rightarrow> Stuck |
     Some ra \<Rightarrow> (
       case ra of
-      Vlong v \<Rightarrow> let rs1 = rs#SP <- nsp in
+      Vlong v \<Rightarrow> let rs1 = rs#(IR SP) <- nsp in
                   Next v rs1 m |
       _ \<Rightarrow> Stuck)
 )"
 
 definition exec_pop :: "usize \<Rightarrow> u64 \<Rightarrow> memory_chunk \<Rightarrow> mem \<Rightarrow> regset \<Rightarrow> ireg \<Rightarrow> outcome" where
 "exec_pop pc sz chunk m rs rd = (
-  let nsp = (rs SP) + (u64_of_memory_chunk chunk) in
-    let addr = (rs SP) in
+  let nsp = (rs (IR SP)) + (u64_of_memory_chunk chunk) in
+    let addr = (rs (IR SP)) in
       case Mem.loadv chunk m (Vptr sp_block addr) of
         None \<Rightarrow> Stuck |
         Some x => 
-          (case x of Vlong v \<Rightarrow> let rs1 =rs # SP <- nsp  in
-          Next (pc + sz) (rs1#rd <- v ) m |
+          (case x of Vlong v \<Rightarrow> let rs1 =rs # (IR SP) <- nsp  in
+          Next (pc + sz) (rs1#(IR rd) <- v ) m |
                      _ \<Rightarrow> Stuck)
 )"
 
 definition exec_push :: "usize \<Rightarrow> u64 \<Rightarrow> memory_chunk \<Rightarrow> mem \<Rightarrow> regset \<Rightarrow> usize \<Rightarrow> outcome" where
 "exec_push pc sz chunk m rs v = ( 
-  let nsp = (rs SP) - (u64_of_memory_chunk chunk) in
+  let nsp = (rs (IR SP)) - (u64_of_memory_chunk chunk) in
       case Mem.storev chunk m (Vptr sp_block nsp) (Vlong v) of
         None \<Rightarrow> Stuck |
-        Some m' => Next (pc + sz) (rs#SP <- nsp) m'
+        Some m' => Next (pc + sz) (rs#(IR SP) <- nsp) m'
 )"
 
+definition of_optbool :: " bool \<Rightarrow> u64" where
+"of_optbool ob = (case ob of True \<Rightarrow> 1 | False \<Rightarrow> 0)"
+
+definition compare_longs :: "u64 \<Rightarrow> u64 \<Rightarrow> regset \<Rightarrow> regset" where
+"compare_longs x y rs = ((((rs#(CR ZF) <- (of_optbool (x = y)))
+                            #(CR CF) <- (of_optbool (x < y)))
+                            #(CR SF) <- (if scast(x-y) <s (0::i64) then 1 else 0))
+                            #(CR OF) <- (sub_overflowi64 x y 0))"
+
+definition eval_testcond :: "testcond \<Rightarrow> regset \<Rightarrow> bool option" where
+"eval_testcond c rs = (
+  case c of
+  Cond_e  \<Rightarrow> (Some (rs (CR ZF) = 1)) | 
+  Cond_ne \<Rightarrow> (Some (rs (CR ZF) = 0)) |
+  Cond_b  \<Rightarrow> (Some (rs (CR CF) = 1)) |
+  Cond_be \<Rightarrow> (Some (rs (CR CF) = 1 \<or> rs (CR ZF) = 1)) |
+  Cond_ae \<Rightarrow> (Some (rs (CR CF) = 0)) |      
+  Cond_a  \<Rightarrow> (Some (rs (CR CF) = 0 \<or> rs (CR ZF) = 0)) |
+  Cond_l  \<Rightarrow> (let n = rs (CR OF); s = rs (CR SF) in 
+             Some ((xor n s) = 1)) |
+  Cond_le \<Rightarrow> (let n = rs (CR OF); s = rs (CR SF); z = rs (CR ZF) in 
+             Some ((xor n s) = 1 \<or> z = 1)) |
+  Cond_ge \<Rightarrow> (let n = rs (CR OF); s = rs (CR SF) in Some ((xor n s) = 0)) |
+  Cond_g  \<Rightarrow> (let n = rs (CR OF); s = rs (CR SF); z = rs (CR ZF) in 
+              Some ((xor n s) = 0 \<and> z = 0)) |
+  Cond_p  \<Rightarrow> (Some (rs (CR PF) = 1)) |
+  Cond_np \<Rightarrow> (Some (rs (CR PF) = 0))
+)"
+
+(*
+definition exec_jcc::"usize \<Rightarrow> u64 \<Rightarrow> regset \<Rightarrow> mem \<Rightarrow> testcond \<Rightarrow> i32 \<Rightarrow> outcome" where
+"exec_jcc pc sz rs m t d \<equiv> 
+  (case eval_testcond t rs of 
+     Some b \<Rightarrow> if b then Next (scast d) rs m 
+     else Next (pc+sz) rs m |
+          None \<Rightarrow> Stuck)"*)
+(*
+definition eval_testcond :: "testcond \<Rightarrow> regset \<Rightarrow> bool option" where
+"eval_testcond c rs = (
+  case c of
+  Cond_e  \<Rightarrow> (case rs (CR ZF) of Vint n \<Rightarrow> Some (n = 1) | _ \<Rightarrow> None) |      
+  Cond_ne \<Rightarrow> (case rs (CR ZF) of Vint n \<Rightarrow> Some (n = 0) | _ \<Rightarrow> None) |
+  Cond_b  \<Rightarrow> (case rs (CR CF) of Vint n \<Rightarrow> Some (n = 1) | _ \<Rightarrow> None) |      
+  Cond_be \<Rightarrow> (case rs (CR CF) of Vint c \<Rightarrow> (
+                case rs (CR ZF) of  Vint z \<Rightarrow> Some (c = 1 \<or> z = 1) |
+                                    _ \<Rightarrow> None) | _ \<Rightarrow> None) |
+  Cond_ae \<Rightarrow> (case rs (CR CF) of Vint n \<Rightarrow> Some (n = 0) | _ \<Rightarrow> None) |      
+  Cond_a  \<Rightarrow> (case rs (CR CF) of Vint c \<Rightarrow> (
+                case rs (CR ZF) of  Vint z \<Rightarrow> Some (c = 0 \<or> z = 0) |
+                                    _ \<Rightarrow> None) | _ \<Rightarrow> None) |
+  Cond_l  \<Rightarrow> (case rs (CR OF) of Vint n \<Rightarrow> (
+                case rs (CR SF) of  Vint s \<Rightarrow> Some ((xor n s) = 1) |
+                                    _ \<Rightarrow> None) | _ \<Rightarrow> None) |
+  Cond_le \<Rightarrow> (case rs (CR OF) of Vint n \<Rightarrow> (
+                case rs (CR SF) of  Vint s \<Rightarrow> (
+                  case rs (CR ZF) of Vint z \<Rightarrow> Some ((xor n s) = 1 \<or> z = 1) | _ \<Rightarrow> None) |
+                                    _ \<Rightarrow> None) | _ \<Rightarrow> None) |
+  Cond_ge \<Rightarrow> (case rs (CR OF) of Vint n \<Rightarrow> (
+                case rs (CR SF) of  Vint s \<Rightarrow> Some ((xor n s) = 0) |
+                                    _ \<Rightarrow> None) | _ \<Rightarrow> None) |
+  Cond_g  \<Rightarrow> (case rs (CR OF) of Vint n \<Rightarrow> (
+                case rs (CR SF) of  Vint s \<Rightarrow> (
+                  case rs (CR ZF) of Vint z \<Rightarrow> Some ((xor n s) = 0 \<and> z = 0) | _ \<Rightarrow> None) |
+                                    _ \<Rightarrow> None) | _ \<Rightarrow> None) |
+  Cond_p  \<Rightarrow> (case rs (CR PF) of Vint n \<Rightarrow> Some (n = 1) | _ \<Rightarrow> None) |
+  Cond_np \<Rightarrow> (case rs (CR PF) of Vint n \<Rightarrow> Some (n = 0) | _ \<Rightarrow> None)
+)"*)
+
+(*Pjmp       d    \<Rightarrow> Next (scast d) rs m*)
 definition exec_instr :: "instruction \<Rightarrow> u64 \<Rightarrow> u64 \<Rightarrow> regset \<Rightarrow> mem \<Rightarrow> outcome" where
 "exec_instr i sz pc rs m = (\<comment> \<open> sz is the binary size (n-byte) of current instruction  \<close>
   case i of
-  Paddq_rr  rd r1 \<Rightarrow> Next (pc + sz) (rs#rd <- ((rs rd) + (rs r1))) m |
+  Paddq_rr  rd r1 \<Rightarrow> Next (pc + sz) ((rs#(IR rd) <- (rs (IR rd) + rs (IR r1)))) m |
   Pret            \<Rightarrow> exec_ret M64 m rs |
   Ppopl     rd    \<Rightarrow> exec_pop pc sz M64 m rs rd |
-  Ppushl_r  r1    \<Rightarrow> exec_push pc sz M64 m rs (rs r1) |
-  Pmovq_rr rd r1  \<Rightarrow> Next (pc + sz) (rs#rd <- (rs r1)) m |
-  Pmulq_r   r1    \<Rightarrow> let rs1 = rs#RAX <- ((rs RAX)*(rs r1)) in
-                     Next (pc + sz) (rs1# RDX <-( (rs RAX)*(rs r1) div (2 ^ 32))) m |
-  Pjmp       d    \<Rightarrow> Next (scast d) rs m
+  Ppushl_r  r1    \<Rightarrow> exec_push pc sz M64 m rs (rs (IR r1)) |
+  Pmovq_rr rd r1  \<Rightarrow> Next (pc + sz) (rs#(IR rd) <- (rs (IR r1))) m |
+  Pmulq_r   r1    \<Rightarrow> let rs1 = rs#(IR RAX) <- ((rs (IR RAX))*(rs (IR r1))) in
+                     Next (pc + sz) (rs1#(IR RDX) <-( (rs (IR RAX))*(rs (IR r1)) div (2 ^ 32))) m |
+  Pjcc      t d    \<Rightarrow> (case eval_testcond t rs of Some b \<Rightarrow> 
+                          if b then Next (scast d) rs m 
+                          else Next (pc+sz) rs m | 
+                        None \<Rightarrow> Stuck) |
+  Pcmpq_rr rd r1 \<Rightarrow> Next (pc+sz)(compare_longs (rs (IR r1)) (rs (IR rd)) rs) m
 )"
 
 
 fun x64_sem :: "nat \<Rightarrow> x64_bin \<Rightarrow> outcome \<Rightarrow> outcome" where
 "x64_sem 0 _ st = st" |
-"x64_sem _ _ Stuck = Stuck" |
+"x64_sem (Suc n) l Stuck = Stuck"|
 "x64_sem (Suc n) l (Next pc rs m) = (
   case x64_decode (unat pc) l of
   None \<Rightarrow> Stuck |
@@ -86,7 +159,7 @@ lemma x64_sem_add_stuck :
   x64_sem n x64_prog (x64_sem m x64_prog Stuck) = xst'"
   apply (cases m,simp)
   subgoal for m
-    apply(cases n,simp)                
+    apply(cases n,simp)              
     by auto
   done
 
@@ -112,7 +185,26 @@ lemma x64_sem_add:
     done
   done
 
+type_synonym hybrid_state = "u64 \<times> outcome"
 
+fun x64_sem1 :: "nat \<Rightarrow> (nat \<times> u64 \<times> x64_bin) list \<Rightarrow> hybrid_state \<Rightarrow> hybrid_state" where
+"x64_sem1 0 _ (pc,st) = (let xst_temp =
+   case st of
+    Next xpc rs m \<Rightarrow> Next 0 rs m |
+    Stuck \<Rightarrow> Stuck in (pc,xst_temp))" |
+"x64_sem1 (Suc n) lt (pc,xst) = (
+  let (num,off,l) = lt!(unat pc) in
+  let pair = 
+    (case xst of Next xpc rs m \<Rightarrow> 
+      if off \<noteq> 0 then 
+        let xst_temp = Next 0 rs m; xst' = x64_sem num l xst_temp in
+        case xst' of Next xpc' rs' m' \<Rightarrow>
+          if rs' (CR ZF) = 1 then (off+pc, xst')
+          else (pc+1, xst')
+      else let xst_temp = Next 0 rs m; xst' = x64_sem num l xst_temp in (pc+1, xst')
+    | Stuck \<Rightarrow> (pc+1,Stuck)) in
+    (x64_sem1 n lt pair))"
+(*
 fun x64_sem1 :: "nat \<Rightarrow> u64 \<Rightarrow> (nat \<times> u64 \<times> x64_bin) list \<Rightarrow> outcome \<Rightarrow> outcome" where
 "x64_sem1 0 _ _ st = (let xst_temp =
    case st of
@@ -124,9 +216,10 @@ fun x64_sem1 :: "nat \<Rightarrow> u64 \<Rightarrow> (nat \<times> u64 \<times> 
     case xst of
     Next xpc rs m \<Rightarrow> Next 0 rs m |
     Stuck \<Rightarrow> Stuck) in
+    if l!0 = 0xE9 then x64_sem1 n (pc+off) lt xst else
   let xst' = x64_sem num l xst_temp in (
     x64_sem1 n (pc+off) lt xst'))"
-
+*)
 
 type_synonym x64_state = outcome
 
