theory/JITPer_add.thy
@@ -13,9 +13,9 @@ lemma aluq_subgoal_rr_aux1:
      prog!(unat pc) = bins \<Longrightarrow>
      sbpf_step prog (SBPF_OK pc rs m) = (SBPF_OK pc' rs' m')  \<Longrightarrow>
      Next spc' reg' xm' = exec_instr xins sz spc reg xm \<Longrightarrow>
-     reg (bpf_to_x64_reg dst) = rs dst \<Longrightarrow>
-     reg (bpf_to_x64_reg src) = rs src \<Longrightarrow>
-     reg' (bpf_to_x64_reg dst) = (rs' dst)"
+     reg (IR (bpf_to_x64_reg dst)) = rs dst \<Longrightarrow>
+     reg (IR (bpf_to_x64_reg src)) = rs src \<Longrightarrow>
+     reg' (IR (bpf_to_x64_reg dst)) = (rs' dst)"
   apply (unfold exec_instr_def step)
   apply simp
   apply(cases "prog ! unat pc",simp_all)
@@ -27,13 +27,13 @@ lemma aluq_subgoal_rr_aux1:
 
 lemma aluq_subgoal_rr_aux2_1:"xins = Paddq_rr dst src \<Longrightarrow> 
   Next pc' reg' m' = exec_instr xins sz pc reg m \<Longrightarrow>
-  \<forall> r \<noteq> dst. reg' r = reg r"
+  \<forall> r \<noteq> dst. reg' (IR r) = reg (IR r)"
   by (simp add: exec_instr_def)
 
 
 lemma aluq_subgoal_rr_aux2:"xins = Paddq_rr (bpf_to_x64_reg dst) (bpf_to_x64_reg src) \<Longrightarrow> 
   Next pc' reg' m' = exec_instr xins sz pc reg m \<Longrightarrow>
-  \<forall> r \<noteq> dst. reg' (bpf_to_x64_reg r) = reg (bpf_to_x64_reg r)"
+  \<forall> r \<noteq> dst. reg' (IR (bpf_to_x64_reg r)) = reg (IR (bpf_to_x64_reg r))"
   using aluq_subgoal_rr_aux2_1 by simp
 
 
@@ -56,7 +56,7 @@ proof-
   a1:"xins = Paddq_rr (bpf_to_x64_reg dst) (bpf_to_x64_reg src) " and
   a2:"match_stack reg m"
   have b0:"bpf_to_x64_reg dst \<noteq> RSP" using bpf_to_x64_reg_def by (cases dst,simp_all)
-  have b1:"reg SP = reg' SP" using exec_instr_def a0 a1 exec_instr_def b0 by simp
+  have b1:"reg (IR SP) = reg' (IR SP)" using exec_instr_def a0 a1 exec_instr_def b0 by simp
   have b2:"m = m'" using a0 a1 exec_instr_def by force
   have "match_stack reg' m'" using b1 b2 a2 match_stack_def by auto
   thus ?thesis by blast
@@ -72,23 +72,23 @@ lemma addq_subgoal_rr_generic:
        a3:"x64_decode 0 l_bin = Some (length l_bin, xins)" and
        a4:"sbpf_step prog (SBPF_OK pc rs m) = (SBPF_OK pc' rs' m')" and
        a5:"Next spc' reg' xm' = exec_instr xins sz spc reg xm" and
-       a6:"match_state (SBPF_OK pc rs m) (Next spc reg xm) " and
+       a6:"match_state (SBPF_OK pc rs m) (pc,(Next spc reg xm)) " and
        a7:"prog!(unat pc) = bins"
-  shows "match_state (SBPF_OK pc' rs' m') (Next spc' reg' xm') "
+  shows "match_state (SBPF_OK pc' rs' m') (pc',(Next spc' reg' xm')) "
 proof -
     have b0:"xins = Paddq_rr (bpf_to_x64_reg dst) (bpf_to_x64_reg src)" 
       using x64_encode_decode_consistency per_jit_add_reg64_1_def a1 a3 list_in_list_prop
     by (smt (verit, ccfv_SIG) Pair_inject map_option_eq_Some option.inject)
-    moreover have b1:"(\<forall> r. (rs r) = reg (bpf_to_x64_reg r))" using a6 spec match_state_def match_reg_def by simp
-    moreover have b2:"(rs src) = reg (bpf_to_x64_reg src)" using a6 spec b1 by simp
-    hence b3:"(rs' dst) = reg' (bpf_to_x64_reg dst)" using aluq_subgoal_rr_aux1 b0 b1 b2 a0 a4 a5 a7 by metis
-    have b4:"\<forall> r \<noteq> dst. reg'(bpf_to_x64_reg r) = reg (bpf_to_x64_reg r)" using b0 a5 aluq_subgoal_rr_aux2 by blast
+    moreover have b1:"(\<forall> r. (rs r) = reg (IR (bpf_to_x64_reg r)))" using a6 spec match_state_def match_reg_def by simp
+    moreover have b2:"(rs src) = reg (IR (bpf_to_x64_reg src))" using a6 spec b1 by simp
+    hence b3:"(rs' dst) = reg' (IR (bpf_to_x64_reg dst))" using aluq_subgoal_rr_aux1 b0 b1 b2 a0 a4 a5 a7 by metis
+    have b4:"\<forall> r \<noteq> dst. reg' (IR (bpf_to_x64_reg r)) = reg (IR (bpf_to_x64_reg r))" using b0 a5 aluq_subgoal_rr_aux2 by blast
     have b5:"\<forall> r \<noteq> dst. (rs' r) = (rs r)" using aluq_subgoal_rr_aux3 a0 a4 a7 by force
-    have b6:"\<forall> r \<noteq> dst. (rs r) = reg ((bpf_to_x64_reg r))" using a6 using b1 by blast
-    have b7:"(\<forall> r \<noteq> dst. (rs' r) = reg' ((bpf_to_x64_reg r)))" using b1 b4 b5 by presburger
+    have b6:"\<forall> r \<noteq> dst. (rs r) = reg (IR (bpf_to_x64_reg r))" using a6 using b1 by blast
+    have b7:"(\<forall> r \<noteq> dst. (rs' r) = reg' (IR (bpf_to_x64_reg r)))" using b1 b4 b5 by presburger
     have b8:"match_stack reg' xm'" using stack_is_not_changed_by_add a6 match_state_def a5 b0 by simp
     have b9:"match_mem m' xm'" using mem_is_not_changed mem_is_not_changed_by_add match_state_def a6
-      by (metis (no_types, lifting) a4 a5 b0 outcome.simps(4) sbpf_state.simps(9))
+      using a4 a5 b0 outcome.simps(4) sbpf_state.simps(9) by fastforce
     (*have b10:"pc = spc" using match_state_def a6 by simp
     have "pc' = pc+1" using a4 a7 a0 
       apply(cases bins,simp_all) 
@@ -99,7 +99,49 @@ proof -
     have "spc' = spc+sz" using a5 apply(unfold exec_instr_def,simp_all) using b0 by(cases xins,simp_all)*)
     thus ?thesis using b3 b7 match_state_def b8 b9 match_reg_def by fastforce
   qed
-      
 
+lemma addq_one_step:
+ assumes a0:"s' = sbpf_step prog s" and
+  a1:"s = (SBPF_OK pc rs m)" and
+  a2:"s' = (SBPF_OK pc' rs' m')" and
+  a3:"xst = (Next xpc xrs xm)" and
+  a4:"match_state s (pc,xst)" and
+  a5:"jitper prog = Some x64_prog" and                      
+  a6:"prog \<noteq> [] \<and> unat pc < length prog \<and> unat pc \<ge> 0" and
+  a7:"xpc = 0" and
+  a8:"prog!(unat pc) = BPF_ALU64 BPF_ADD dst (SOReg src)" 
+shows "\<exists> xst'. x64_sem1 1 x64_prog (pc,xst) = (pc',xst') \<and> 
+  match_state s' (pc',xst')"
+  proof-
+    let "?bpf_ins" = "prog!(unat pc)"
+    let "?l_bin"= "snd (snd (the (per_jit_ins ?bpf_ins)))"
+    have c0:"?l_bin = snd (snd (the (per_jit_add_reg64_1 dst src)))" using a8 by fastforce
+    have c1:"?l_bin = x64_encode (Paddq_rr (bpf_to_x64_reg dst) (bpf_to_x64_reg src))" using per_jit_add_reg64_1_def c0 by fastforce
+    have c2:"snd (snd(x64_prog!(unat pc))) = ?l_bin" using a6 c0 a5 aux5 by metis
+    let "?st" = "x64_sem (fst (x64_prog!(unat pc))) ?l_bin xst"
+    have "x64_prog!(unat pc) = the (per_jit_ins ?bpf_ins)" using aux5 a5 a6 by blast
+    then have c3_0:"x64_prog!(unat pc) = the (per_jit_add_reg64_1 dst src)" using a8 by simp
+
+    have "\<exists> num off l. x64_prog!(unat pc) = (num,off,l)" by (metis split_pairs)
+    then obtain num off l where c_aux:"x64_prog!(unat pc) = (num,off,l)" by auto
+
+    then have c3_1:"num = 1" using per_jit_add_reg64_1_def c3_0 by simp
+    moreover have "list_in_list ?l_bin 0 ?l_bin" using  list_in_list_prop by simp
+    hence "\<exists> xins2. x64_decode 0 ?l_bin = Some (length ?l_bin, xins2) " 
+      using x64_encode_decode_consistency a3 a7 c1 list_in_list_prop c3_1 by blast
+    then obtain xins2 where c3:"x64_decode 0 ?l_bin = Some (length ?l_bin, xins2)" by auto
+    have c4:"?st = exec_instr xins2 (of_nat (length ?l_bin)) xpc xrs xm" using c3 a8 a3 a7 c_aux
+      apply(cases xst,simp_all) apply(cases "prog ! unat pc",simp_all) by (simp add: calculation)
+    have c5:"xins2 = Paddq_rr (bpf_to_x64_reg dst) (bpf_to_x64_reg src)" using Pair_inject c4 c3 c1 option.inject x64_encode_decode_consistency list_in_list_prop by metis
+    have c6:"\<exists> xrs' xpc' xm'. ?st = Next xpc' xrs' xm'" using exec_instr_def spec c5 c4 by auto
+    obtain xrs' xpc' xm' where c7:"?st = Next xpc' xrs' xm'" using c6 by auto
+    have c8:"x64_sem num l xst = ?st \<and> match_state s' (pc',?st)"  
+      using addq_subgoal_rr_generic a0 a1 a2 c7 a4 a3 per_jit_add_reg64_1_def a8 c4 c3 c2 c_aux by force
+    (*have c8:"match_state s' (pc',?st)" using addq_subgoal_rr_generic a0 a1 a2 c7 a4 a3 per_jit_add_reg64_1_def b2 c4 c3 True by fastforce*)
+    have c9_1:"off = 0" using c_aux corr_pc_aux1_1 a5 a6 a8 by fastforce
+    have "x64_sem1 1 x64_prog (pc,xst) = (pc',(Next 0 xrs' xm')) \<and> match_state s' (pc', Next 0 xrs' xm')" 
+      using a8 c9_1  a0 a1 a2 a3 a5 a6 a7 x64_sem1_pc_aux1 c7 c8 c_aux by (metis insertCI match_state_eqiv)
+    thus ?thesis by simp
+  qed
 
 end
