theory/JITPer_jump.thy
@@ -3,11 +3,122 @@ imports
   Main
   rBPFCommType rBPFSyntax rBPFSem
   x64Syntax x64Semantics x64Assembler
-  JITPer_aux
+  JITPer_aux Proof1
 
 begin
 
-lemma ja_subgoal_rr_generic:
+
+lemma jccq_subgoal_rr_aux3:"bins = BPF_JUMP cond dst (SOReg src) d \<Longrightarrow> 
+  sbpf_step prog (SBPF_OK pc rs m) = (SBPF_OK pc' rs' m') \<Longrightarrow> 
+  prog!(unat pc) = bins \<Longrightarrow>
+  \<forall> r. rs' r = rs r"
+  apply(cases bins,simp_all)
+  apply(cases "prog ! unat pc", simp_all)
+  subgoal for x161 by(simp split:if_split_asm) 
+  done
+
+
+lemma jcc_subgoal_rr_generic:
+  assumes a0:"bins = BPF_JUMP cond dst (SOReg src) d" and
+       a1:"per_jit_jcc cond dst src (scast d) = Some (num, off, l_bin)" and
+       a3:"x64_decode 0 l_bin = Some (n, xins)" and
+       a4:"sbpf_step prog (SBPF_OK pc rs m) = (SBPF_OK pc' rs' m')" and
+       a5:"Next spc' reg' xm' = exec_instr xins sz spc reg xm" and
+       a6:"match_state (SBPF_OK pc rs m) (pc, Next spc reg xm) " and
+       a7:"prog!(unat pc) = bins" and
+       a8:"cond = Eq"
+  shows "match_state (SBPF_OK pc' rs' m') (pc', Next spc' reg' xm') "
+proof -
+  let "?tcond" = "Cond_e"
+  have b0_1:"l_bin = (let ins1 = Pcmpq_rr (bpf_to_x64_reg dst) (bpf_to_x64_reg src) in
+      let ins2 = (Pjcc ?tcond 0) in x64_encode ins1@x64_encode ins2)" using a8 per_jit_jcc_def a1 a3 by simp 
+  let "?l_bin1" = "x64_encode (Pcmpq_rr (bpf_to_x64_reg dst) (bpf_to_x64_reg src))"
+  let "?l_bin2" = "x64_encode (Pjcc ?tcond 0)"
+  have d0:"list_in_list (?l_bin1@?l_bin2) (0::nat) l_bin" using list_in_list_prop b0_1 by metis
+  have d0_0:"list_in_list l_bin 0 l_bin = list_in_list ?l_bin1 0 l_bin \<and> list_in_list ?l_bin2 (0 + length ?l_bin1) l_bin" 
+       using list_in_list_concat d0 b0_1 list_in_list_prop by blast
+  have d0_1:"list_in_list ?l_bin1 0 l_bin" using d0 d0_0 by auto
+  hence b0:"xins = Pcmpq_rr (bpf_to_x64_reg dst) (bpf_to_x64_reg src)"
+      using x64_encode_decode_consistency a3 by (metis Pair_inject option.sel)
+    
+  moreover have b1:"(\<forall> r. (rs r) = reg (IR (bpf_to_x64_reg r)))" using a6 spec match_state_def match_reg_def by simp
+  have b2:"\<forall> r. reg' (IR (bpf_to_x64_reg r)) = reg (IR (bpf_to_x64_reg r))" using b0 a5 by (simp add: exec_instr_def compare_longs_def)
+  have b3:"\<forall> r. (rs' r) = (rs r)" using a0 a4 a7 jccq_subgoal_rr_aux3 by blast
+  have b4:"(\<forall> r. (rs' r) = reg' (IR (bpf_to_x64_reg r)))" using b1 b2 b3 by presburger
+  have b8:"match_stack reg' xm'" using a6 match_state_def a5 b0 apply (simp add: exec_instr_def compare_longs_def) by(simp add:match_stack_def)
+  have b9:"match_mem m' xm'" using match_state_def a6 a5 b0 apply (simp add: exec_instr_def) 
+    using a4 mem_is_not_changed by blast
+  thus ?thesis using b4  match_state_def b8 b9 match_reg_def by fastforce
+qed
+
+lemma jump_one_step:
+  assumes a0:"s' = sbpf_step prog s" and
+  a1:"s = (SBPF_OK pc rs m)" and
+  a2:"s' = (SBPF_OK pc' rs' m')" and
+  a3:"xst = (Next xpc xrs xm)" and
+  a4:"match_state s (pc,xst)" and
+  a5:"jitper prog = Some x64_prog" and                      
+  a6:"prog \<noteq> [] \<and> unat pc < length prog \<and> unat pc \<ge> 0" and
+  a7:"xpc = 0" and
+  a8:"prog!(unat pc) = BPF_JUMP cond dst (SOReg src) x"
+shows "\<exists> xst'. x64_sem1 1 x64_prog (pc,xst) = (pc',xst') \<and> 
+  match_state s' (pc',xst')"
+proof-
+    let "?bpf_ins" = "prog!(unat pc)"
+    let "?l_bin"= "snd (snd (the (per_jit_ins ?bpf_ins)))"
+    have c1_0:"?l_bin = snd (snd (the (per_jit_jcc cond dst src (scast x))))" using a8 by auto
+    let "?tcond" = "Cond_e"
+    have c1_1:"cond = Eq" sorry
+    have c1:"?l_bin = (let ins1 = Pcmpq_rr (bpf_to_x64_reg dst) (bpf_to_x64_reg src); ins2 = (Pjcc ?tcond 0) in x64_encode ins1@x64_encode ins2 )" 
+      using c1_1 per_jit_jcc_def c1_0 by simp
+    have c0:"?l_bin = snd (snd (the (per_jit_jcc cond dst src (scast x))))" using a8 by fastforce
+
+    have "\<exists> num off l. x64_prog!(unat pc) = (num,off,l)" by (metis split_pairs)
+    then obtain num off l where c_aux:"x64_prog!(unat pc) = (num,off,l)" by auto
+
+    have c2:"l = ?l_bin" using a6 c0 a5 aux5 c_aux by fastforce
+    let "?st" = "x64_sem num ?l_bin xst"
+    have "x64_prog!(unat pc) = the (per_jit_ins ?bpf_ins)" using aux5 a5 a6 by blast
+    then have c3:"x64_prog!(unat pc) = the (per_jit_jcc cond dst src (scast x))" using a8 by simp
+    then have c3_1:"num = 1" using per_jit_jcc_def c1_1 c_aux by simp
+
+    let "?l_bin1" = "x64_encode (Pcmpq_rr (bpf_to_x64_reg dst) (bpf_to_x64_reg src))"
+    let "?l_bin2" = "x64_encode (Pjcc ?tcond 0)"
+    have d0:"list_in_list (?l_bin1@?l_bin2) (0::nat) ?l_bin" using list_in_list_prop c1 by metis
+    have d0_0:"list_in_list ?l_bin 0 ?l_bin = list_in_list ?l_bin1 0 ?l_bin \<and> list_in_list ?l_bin2 (0 + length ?l_bin1) ?l_bin" 
+       using list_in_list_concat d0 c1 list_in_list_prop by blast
+    have d0_1:"list_in_list ?l_bin1 0 ?l_bin" using d0 d0_0 by auto
+    have d0_2:"list_in_list ?l_bin2 (0+length ?l_bin1) ?l_bin" using d0 d0_0 by auto
+    hence "\<exists> xins1 sz1. x64_decode 0 ?l_bin = Some (sz1, xins1)" 
+      by (metis c1 d0 list_in_list_concat x64_encode_decode_consistency)
+    then obtain xins1 sz1 where d1:"x64_decode 0 ?l_bin = Some (sz1, xins1)" by auto
+    have d2:"(sz1,xins1) = (3, Pcmpq_rr (bpf_to_x64_reg dst) (bpf_to_x64_reg src))"  using d0_1 x64_encode_decode_consistency d1 by fastforce
+    have c4:"?st = exec_instr xins1 (of_nat sz1) xpc xrs xm" using c3_1 d2 c1 c2 a7 a3 d1 by auto 
+    have c6:"\<exists> xrs' xpc' xm'. ?st = Next xpc' xrs' xm'" using exec_instr_def spec c4 d2 by simp
+    obtain xrs' xpc' xm' where c7:"?st = Next xpc' xrs' xm'" using c6 by auto
+    have cn:"x64_sem num l xst = ?st \<and> match_state s' (pc',?st)" 
+      using jcc_subgoal_rr_generic a0 a1 a2 c7 a4 a3 per_jit_jcc_def a8 c4 c1_1 d1 c2 c7 by force
+    
+    have "exec_instr xins1 (of_nat sz1) xpc xrs xm = Next (xpc+(of_nat sz1))(compare_longs (xrs (IR (bpf_to_x64_reg src))) (xrs (IR (bpf_to_x64_reg dst))) xrs) xm"
+      using  exec_instr_def d2 a3 by simp
+     
+    hence e0:"let x = xrs (IR (bpf_to_x64_reg src)); y = xrs (IR (bpf_to_x64_reg dst)) in
+     xrs' = ((((xrs#(CR ZF) <- (of_optbool (x = y)))
+                            #(CR CF) <- (of_optbool (x < y)))
+                            #(CR SF) <- (if scast(x-y) <s (0::i64) then 1 else 0))
+                            #(CR OF) <- (sub_overflowi64 x y 0))"
+      using c7 c4 d2 c4 a3 exec_instr_def of_optbool_def a8
+      by (simp add: compare_longs_def)    
+    hence e1:"xrs (IR (bpf_to_x64_reg dst)) = xrs (IR (bpf_to_x64_reg src)) \<longrightarrow>xrs' (CR ZF) = 1" by (smt (verit, del_insts) crbit.distinct(1) crbit.distinct(5) crbit.distinct(7)  fun_upd_apply preg.inject(2) x64Semantics.of_optbool_def)
+    have e2:"xrs (IR (bpf_to_x64_reg dst)) \<noteq> xrs (IR (bpf_to_x64_reg src)) \<longrightarrow>xrs' (CR ZF) = 0" by (smt (verit, del_insts) crbit.distinct(1) crbit.distinct(5) crbit.distinct(7) e0 fun_upd_apply preg.inject(2) x64Semantics.of_optbool_def)
+    have e3_0:"off = scast x + 1" using c_aux per_jit_jcc_def c3 c1_1 by simp
+    have e3:"off\<noteq>0" sorry
+    have "x64_sem1 1 x64_prog (pc,xst) = (pc', Next 0 xrs' xm')"
+      using a8 e1 e2 cn a0 a1 a2 a3 a4 a5 a6 a7 x64_sem1_pc_aux1 c_aux match_state_eqiv e3 c7 x64_sem1_pc_aux2 by auto
+    then show ?thesis using a8 c2 match_state_eqiv c7 cn by fastforce
+    qed
+
+(*lemma ja_subgoal_rr_generic:
   assumes a0:"bins = BPF_JA d" and
        a1:"per_jit_ja (scast d) = Some (n, off, l_bin)" and
        a3:"x64_decode 0 l_bin = Some (length l_bin, xins)" and
@@ -29,6 +140,6 @@ proof -
     have b9:"match_mem m' xm'" using match_state_def a6 a5 b0 apply (simp add: exec_instr_def) 
       using a4 mem_is_not_changed by blast
     thus ?thesis using b4  match_state_def b8 b9 match_reg_def by fastforce
-  qed
+  qed*)
       
 end
